src/Std/Data/Iterators/Combinators/Monadic/Zip.lean
@@ -313,6 +313,10 @@ instance Zip.instProductive [Monad m] [Productive α₁ m] [Productive α₂ m] 
     Productive (Zip α₁ m α₂ β₂) m :=
   Productive.of_productivenessRelation Zip.instProductivenessRelation
 
+instance Zip.instIteratorLoopNew [Monad m] :
+    IteratorLoopNew (Zip α₁ m α₂ β₂) m n :=
+  .defaultImplementation
+
 instance Zip.instIteratorLoop [Monad m] [Monad n] :
     IteratorLoop (Zip α₁ m α₂ β₂) m n :=
   .defaultImplementation
